Given the number of questions across the sections in the images, I'll provide solutions for each question in a step-by-step manner. Since there are many questions, I’ll divide the answers into several responses to keep things organized. Let's start with **Section A**.

### Section A

1. **If \( A = \{2, 3, 4, 5\} \) and \( B = \{0, 1, 2, 3\} \), find \( A \cap B \).**
   - **Solution**: The intersection \( A \cap B \) consists of elements that are in both sets \( A \) and \( B \).
   - \( A \cap B = \{2, 3\} \).

2. **If \( A = \{1, 2, 3\} \), \( B = \{3, 4, 5\} \) and \( C = \{0, 2, 3\} \), find \( (A \cap B) \times C \).**
   - **Solution**: First, find the intersection \( A \cap B \):
     - \( A \cap B = \{3\} \).
     - Now, \( (A \cap B) \times C = \{3\} \times \{0, 2, 3\} \).
     - This results in \( \{(3, 0), (3, 2), (3, 3)\} \).

3. **Define Tautology.**
   - **Solution**: A tautology is a formula that is true in every possible interpretation. In propositional logic, a tautology is a statement that is always true regardless of the truth values of its constituent propositions.
     - Example: \( p \vee \neg p \) (where \( p \) is a proposition) is a tautology because either \( p \) is true, or \( \neg p \) (not \( p \)) is true.

4. **Define Scalar matrix with an example.**
   - **Solution**: A scalar matrix is a diagonal matrix in which all the diagonal elements are equal.
     - Example: \( \begin{pmatrix} 3 & 0 & 0 \\ 0 & 3 & 0 \\ 0 & 0 & 3 \end{pmatrix} \) is a scalar matrix where all diagonal elements are 3.

5. **If \( A = \begin{pmatrix} 3 & 2 \\ -1 & 4 \end{pmatrix} \) and \( B = \begin{pmatrix} 3 & 5 \\ -2 & 4 \end{pmatrix} \), find \( 2A + 3B \).**
   - **Solution**:
     - \( 2A = 2 \times \begin{pmatrix} 3 & 2 \\ -1 & 4 \end{pmatrix} = \begin{pmatrix} 6 & 4 \\ -2 & 8 \end{pmatrix} \).
     - \( 3B = 3 \times \begin{pmatrix} 3 & 5 \\ -2 & 4 \end{pmatrix} = \begin{pmatrix} 9 & 15 \\ -6 & 12 \end{pmatrix} \).
     - \( 2A + 3B = \begin{pmatrix} 6 & 4 \\ -2 & 8 \end{pmatrix} + \begin{pmatrix} 9 & 15 \\ -6 & 12 \end{pmatrix} = \begin{pmatrix} 15 & 19 \\ -8 & 20 \end{pmatrix} \).

6. **Find the characteristic roots of the matrix \( A = \begin{pmatrix} 1 & 2 \\ 3 & 2 \end{pmatrix} \).**
   - **Solution**:
     - The characteristic equation is \( \text{det}(A - \lambda I) = 0 \).
     - \( A - \lambda I = \begin{pmatrix} 1-\lambda & 2 \\ 3 & 2-\lambda \end{pmatrix} \).
     - Determinant: \( (1-\lambda)(2-\lambda) - 6 = \lambda^2 - 3\lambda - 4 \).
     - Solve \( \lambda^2 - 3\lambda - 4 = 0 \) to find roots: \( \lambda = 4 \) or \( \lambda = -1 \).

7. **If \( \log_7 x_1 + \log_7 x_2 + \log_7 x_3 = 6 \), find \( x \).**
   - **Solution**:
     - \( \log_7 (x_1 x_2 x_3) = 6 \).
     - \( x_1 x_2 x_3 = 7^6 \).
     - So, \( x = \sqrt[3]{7^6} = 7^2 = 49 \).

8. **Define permutation and combination.**
   - **Solution**:
     - **Permutation**: The arrangement of objects in a specific order. The number of ways to arrange \( n \) objects taken \( r \) at a time is given by \( P(n, r) = \frac{n!}{(n-r)!} \).
     - **Combination**: The selection of objects without regard to order. The number of ways to choose \( r \) objects from \( n \) objects is given by \( C(n, r) = \frac{n!}{r!(n-r)!} \).

9. **Define an abelian group.**
   - **Solution**: An abelian group is a group in which the group operation is commutative, i.e., for all elements \( a \) and \( b \) in the group, \( a \ast b = b \ast a \).

10. **If \( \vec{a} = 2\hat{i} + 3\hat{j} - 4\hat{k} \), \( \vec{b} = 3\hat{i} - 4\hat{j} - 5\hat{k} \), find \( |\vec{a} + \vec{b}| \).**
    - **Solution**:
      - \( \vec{a} + \vec{b} = (2+3)\hat{i} + (3-4)\hat{j} + (-4-5)\hat{k} = 5\hat{i} - \hat{j} - 9\hat{k} \).
      - \( |\vec{a} + \vec{b}| = \sqrt{(5)^2 + (-1)^2 + (-9)^2} = \sqrt{25 + 1 + 81} = \sqrt{107} \).

11. **Find the distance between the point \( A = (-7, 4) \) and \( B = (-5, -1) \).**
    - **Solution**:
      - Distance \( d = \sqrt{(-7 + 5)^2 + (4 + 1)^2} = \sqrt{(-2)^2 + (5)^2} = \sqrt{4 + 25} = \sqrt{29} \).

12. **Find the equation of the line whose y-intercept is -2 and slope is \( \frac{3}{2} \).**
    - **Solution**:
      - The equation of a line in slope-intercept form is \( y = mx + c \), where \( m \) is the slope and \( c \) is the y-intercept.
      - Here, \( y = \frac{3}{2}x - 2 \).

### Section B

 Let's solve **Section B**:

### Section B

1. **Find the radius of the circle \( x^2 + y^2 + 6x - 4y - 12 = 0 \).**
   - **Solution**:
     - Rewrite the equation in standard form: \( (x^2 + 6x) + (y^2 - 4y) = 12 \).
     - Complete the square:
       - \( x^2 + 6x = (x + 3)^2 - 9 \).
       - \( y^2 - 4y = (y - 2)^2 - 4 \).
     - So, the equation becomes:
       - \( (x + 3)^2 + (y - 2)^2 = 25 \).
     - The radius is \( \sqrt{25} = 5 \).

2. **Find the equation of the circle whose center is (2, -3) and radius 4.**
   - **Solution**:
     - The standard form of a circle’s equation is \( (x - h)^2 + (y - k)^2 = r^2 \), where \( (h, k) \) is the center and \( r \) is the radius.
     - Plugging in the values:
       - \( (x - 2)^2 + (y + 3)^2 = 16 \).

3. **If \( x + y + z = 0 \), show that \( x^3 + y^3 + z^3 = 3xyz \).**
   - **Solution**:
     - The identity \( x^3 + y^3 + z^3 - 3xyz = (x + y + z)(x^2 + y^2 + z^2 - xy - yz - zx) \) holds true.
     - Since \( x + y + z = 0 \), the right-hand side becomes 0.
     - Thus, \( x^3 + y^3 + z^3 = 3xyz \).

4. **Solve \( x^2 + 4x + 4 = 0 \).**
   - **Solution**:
     - Factorize the quadratic equation:
       - \( x^2 + 4x + 4 = (x + 2)^2 = 0 \).
       - \( x + 2 = 0 \) implies \( x = -2 \).

5. **Solve \( \frac{x}{x + 1} - \frac{x - 1}{x} = 1 \).**
   - **Solution**:
     - Find a common denominator:
       - \( \frac{x(x) - (x-1)(x+1)}{x(x+1)} = 1 \).
       - Simplify: \( \frac{x^2 - (x^2 - 1)}{x(x + 1)} = 1 \).
       - \( \frac{1}{x(x + 1)} = 1 \).
       - \( 1 = x(x + 1) \).
       - \( x^2 + x - 1 = 0 \).
     - Solve using the quadratic formula:
       - \( x = \frac{-1 \pm \sqrt{1 + 4}}{2} = \frac{-1 \pm \sqrt{5}}{2} \).
       - So, \( x = \frac{-1 + \sqrt{5}}{2} \) or \( x = \frac{-1 - \sqrt{5}}{2} \).

6. **Solve \( 2\cos^2\theta + 3\sin\theta = 0 \).**
   - **Solution**:
     - Rewrite \( \cos^2\theta \) using \( \sin^2\theta = 1 - \cos^2\theta \):
       - \( 2(1 - \sin^2\theta) + 3\sin\theta = 0 \).
       - \( 2 - 2\sin^2\theta + 3\sin\theta = 0 \).
       - \( 2\sin^2\theta - 3\sin\theta - 2 = 0 \).
     - Let \( x = \sin\theta \). Solve the quadratic equation:
       - \( 2x^2 - 3x - 2 = 0 \).
       - Solve using the quadratic formula:
         - \( x = \frac{-(-3) \pm \sqrt{(-3)^2 - 4(2)(-2)}}{2(2)} \).
         - \( x = \frac{3 \pm \sqrt{9 + 16}}{4} \).
         - \( x = \frac{3 \pm \sqrt{25}}{4} \).
         - \( x = \frac{3 \pm 5}{4} \).
       - \( x = 2 \) (which is not possible for \( \sin\theta \)) or \( x = -\frac{1}{2} \).
       - So, \( \sin\theta = -\frac{1}{2} \).
       - \( \theta = 210^\circ \) or \( \theta = 330^\circ \).

7. **If \( y = e^{2x} \), find \( \frac{dy}{dx} \).**
   - **Solution**:
     - Differentiate \( y \) with respect to \( x \):
       - \( \frac{dy}{dx} = 2e^{2x} \).

8. **Find the area of the triangle whose vertices are \( A(1, 2) \), \( B(3, 5) \), and \( C(4, 1) \).**
   - **Solution**:
     - Use the formula for the area of a triangle with vertices \( (x_1, y_1) \), \( (x_2, y_2) \), and \( (x_3, y_3) \):
       - Area \( = \frac{1}{2} \left| x_1(y_2 - y_3) + x_2(y_3 - y_1) + x_3(y_1 - y_2) \right| \).
       - Substitute the given points:
         - \( \text{Area} = \frac{1}{2} \left| 1(5 - 1) + 3(1 - 2) + 4(2 - 5) \right| \).
         - \( \text{Area} = \frac{1}{2} \left| 4 + (-3) + (-12) \right| = \frac{1}{2} \times 11 = \frac{11}{2} \).

9. **Find \( \frac{dy}{dx} \) if \( y = \sin^{-1}(2x) \).**
   - **Solution**:
     - Differentiate \( y \) with respect to \( x \) using the chain rule:
       - \( \frac{dy}{dx} = \frac{2}{\sqrt{1 - 4x^2}} \).

10. **Integrate \( \int \frac{dx}{x \ln x} \).**
    - **Solution**:
      - Let \( u = \ln x \), then \( du = \frac{dx}{x} \).
      - The integral becomes \( \int \frac{du}{u} = \ln|u| + C = \ln|\ln x| + C \).

11. **Evaluate \( \int_{0}^{1} x e^{2x} dx \).**
    - **Solution**:
      - Use integration by parts where \( u = x \) and \( dv = e^{2x}dx \).
      - \( du = dx \) and \( v = \frac{e^{2x}}{2} \).
      - The integral becomes:
        - \( \left[ \frac{x e^{2x}}{2} \right]_0^1 - \int_0^1 \frac{e^{2x}}{2} dx \).
        - \( = \frac{e^2}{2} - \frac{1}{4}e^{2x} \Big|_0^1 = \frac{e^2}{2} - \frac{e^2 - 1}{4} \).
        - Simplify: \( = \frac{e^2}{2} - \frac{e^2}{4} + \frac{1}{4} = \frac{e^2}{4} + \frac{1}{4} \).

12. **Evaluate \( \int_0^\pi \sin^2 x dx \).**
    - **Solution**:
      - Use the identity \( \sin^2 x = \frac{1 - \cos(2x)}{2} \):
        - \( \int_0^\pi \sin^2 x dx = \frac{1}{2} \int_0^\pi (1 - \cos(2x)) dx \).
        - \( = \frac{1}{2} \left[ x - \frac{\sin(2x)}{2} \right]_0^\pi \).
        - \( = \frac{1}{2} \left[ \pi - 0 \right] = \frac{\pi}{2} \).

### Section C
 Let's solve **Section C**:

### Section C

1. **Find the equation of the straight line passing through the point \( (3, 2) \) and perpendicular to the line \( 3x + 4y - 7 = 0 \).**
   - **Solution**:
     - The slope of the given line \( 3x + 4y - 7 = 0 \) is \( -\frac{3}{4} \) (since the slope \( m \) is \( -\frac{A}{B} \) for a line \( Ax + By + C = 0 \)).
     - The slope of the line perpendicular to this will be the negative reciprocal, which is \( \frac{4}{3} \).
     - The equation of the line in point-slope form is:
       - \( y - 2 = \frac{4}{3}(x - 3) \).
     - Simplifying, we get:
       - \( 3(y - 2) = 4(x - 3) \).
       - \( 3y - 6 = 4x - 12 \).
       - \( 4x - 3y - 6 = 0 \).

2. **Find the center and radius of the circle \( x^2 + y^2 + 8x - 10y + 20 = 0 \).**
   - **Solution**:
     - Rewrite the equation by completing the square:
       - \( x^2 + 8x + y^2 - 10y = -20 \).
       - \( (x + 4)^2 - 16 + (y - 5)^2 - 25 = -20 \).
       - \( (x + 4)^2 + (y - 5)^2 = 21 \).
     - The center is \( (-4, 5) \) and the radius is \( \sqrt{21} \).

3. **If \( \theta \) is the angle between the vectors \( \vec{a} = 2\hat{i} + 3\hat{j} + 4\hat{k} \) and \( \vec{b} = \hat{i} - 2\hat{j} + 3\hat{k} \), find \( \cos \theta \).**
   - **Solution**:
     - Use the formula for the dot product:
       - \( \vec{a} \cdot \vec{b} = 2(1) + 3(-2) + 4(3) = 2 - 6 + 12 = 8 \).
     - The magnitudes of \( \vec{a} \) and \( \vec{b} \) are:
       - \( |\vec{a}| = \sqrt{2^2 + 3^2 + 4^2} = \sqrt{4 + 9 + 16} = \sqrt{29} \).
       - \( |\vec{b}| = \sqrt{1^2 + (-2)^2 + 3^2} = \sqrt{1 + 4 + 9} = \sqrt{14} \).
     - \( \cos \theta = \frac{\vec{a} \cdot \vec{b}}{|\vec{a}| |\vec{b}|} = \frac{8}{\sqrt{29} \cdot \sqrt{14}} = \frac{8}{\sqrt{406}} \).

4. **Solve \( \tan^{-1}x + \tan^{-1}y = \frac{\pi}{4} \).**
   - **Solution**:
     - Use the identity: \( \tan^{-1}a + \tan^{-1}b = \tan^{-1}\left(\frac{a + b}{1 - ab}\right) \).
     - So, \( \frac{x + y}{1 - xy} = 1 \).
     - This implies \( x + y = 1 - xy \), or \( xy + x + y = 1 \).
     - Factor the equation: \( (x + 1)(y + 1) = 2 \).
     - The solution involves finding \( x \) and \( y \) such that this equation holds.

5. **Solve \( 2\cos^2 x - 3\cos x + 1 = 0 \).**
   - **Solution**:
     - Let \( u = \cos x \).
     - The equation becomes \( 2u^2 - 3u + 1 = 0 \).
     - Factorize: \( (2u - 1)(u - 1) = 0 \).
     - So, \( u = \frac{1}{2} \) or \( u = 1 \).
     - If \( \cos x = \frac{1}{2} \), then \( x = \frac{\pi}{3} \) or \( x = \frac{5\pi}{3} \).
     - If \( \cos x = 1 \), then \( x = 0 \).

6. **Find the area bounded by the curves \( y^2 = 4x \) and \( x^2 = 4y \).**
   - **Solution**:
     - First, solve the points of intersection:
       - \( y^2 = 4x \) and \( x^2 = 4y \).
     - Substitute \( x = \frac{y^2}{4} \) into \( x^2 = 4y \):
       - \( \left(\frac{y^2}{4}\right)^2 = 4y \).
       - \( \frac{y^4}{16} = 4y \).
       - \( y^4 = 64y \) implies \( y(y^3 - 64) = 0 \).
       - \( y = 0 \) or \( y = 4 \).
     - The corresponding \( x \) values are \( x = 0 \) and \( x = 4 \).
     - Integrate the area between the curves:
       - Find the area by subtracting the lower curve from the upper curve between the points of intersection.

 
